Add: generalize context & Skolemization typeclass, add branching example

theories/Proofs.v
@@ -7,52 +7,58 @@ From Tableaux Require Import Syntax.
 Section TableauxProofs.
   Context `{set_nat : set nat} {pred func var : Atom} (sko : Skolemization_ pred func var).
 
+  Existing Instance fv_ctx.
+
   Let set_var := set_atom var.
   Let set_func := set_atom func.
+  Let Con := Con_ pred func var.
+  Let Term := Term_ func var.
+  Let Form := Form_ pred func var.
+  Let sko_record := sko_record sko.
 
   Inductive hasTableau_
-    : Con_ pred func var -> set_var -> set_func -> Substitution var (Term_ func var) -> Prop :=
+    : Con -> set_var -> sko_record -> Substitution var Term -> Prop :=
 
   (** Axioms *)
   | hasTableauBot :
-    forall (Gamma : Con_ pred func var) (S : set_var) (Sf : set_func) (sigma : Substitution var (Term_ func var)),
+    forall (Gamma : Con) (S : set_var) (Sf : sko_record) (sigma : Substitution var Term),
       (Bot \in Gamma) -> hasTableau_ Gamma S Sf sigma
   | hasTableauContr :
-    forall (Gamma : Con_ pred func var) (S : set_var) (Sf : set_func) (sigma : Substitution var (Term_ func var))
-      (P P' : Form_ pred func var), (P \in Gamma) -> (P' \in Gamma) -> Neg P@[sigma] = P'@[sigma] -> hasTableau_ Gamma S Sf sigma
+    forall (Gamma : Con) (S : set_var) (Sf : sko_record) (sigma : Substitution var Term)
+      (P P' : Form), (P \in Gamma) -> (P' \in Gamma) -> Neg P@[sigma] = P'@[sigma] -> hasTableau_ Gamma S Sf sigma
 
   (** Alpha rules *)
   | hasTableauNegNeg :
-    forall (Gamma : Con_ pred func var) (S : set_var) (Sf : set_func) (sigma : Substitution var (Term_ func var))
-      (F : Form_ pred func var), Neg (Neg F) \in Gamma -> hasTableau_ (Gamma ,, F) S Sf sigma -> hasTableau_ Gamma S Sf sigma
+    forall (Gamma : Con) (S : set_var) (Sf : sko_record) (sigma : Substitution var Term)
+      (F : Form), Neg (Neg F) \in Gamma -> hasTableau_ (Gamma ,, F) S Sf sigma -> hasTableau_ Gamma S Sf sigma
   | hasTableauNegOr :
-    forall (Gamma : Con_ pred func var) (S : set_var) (Sf : set_func) (sigma : Substitution var (Term_ func var))
-      (F1 F2 : Form_ pred func var),
+    forall (Gamma : Con) (S : set_var) (Sf : sko_record) (sigma : Substitution var Term)
+      (F1 F2 : Form),
       Neg (Or F1 F2) \in Gamma -> hasTableau_ (Gamma ,, Neg F1 ,, Neg F2) S Sf sigma -> hasTableau_ Gamma S Sf sigma
 
-  (** Beta rule *)
+  (** Beta rule *) (* TODO: JOIN CONDITION IN SKOLEMIZATION *)
   | hasTableauOr :
-    forall (Gamma : Con_ pred func var) (S1 S2 : set_var) (Sf1 Sf2 : set_func) (sigma : Substitution var (Term_ func var))
-      (F1 F2 : Form_ pred func var),
+    forall (Gamma : Con) (S1 S2 : set_var) (Sf1 Sf2 : sko_record) (sigma : Substitution var Term)
+      (F1 F2 : Form),
       (Or F1 F2) \in Gamma -> hasTableau_ (Gamma ,, F1) S1 Sf1 sigma -> hasTableau_ (Gamma ,, F2) S2 Sf2 sigma ->
-      disjoint S1 S2 -> disjoint Sf1 Sf2 -> hasTableau_ Gamma (S1 \union S2) (Sf1 \union Sf2) sigma
+      disjoint S1 S2 -> hasTableau_ Gamma (S1 \union S2) (join Sf1 Sf2) sigma
 
   (** Gamma rule *)
   | hasTableauAll :
-    forall (Gamma : Con_ pred func var) (S : set_var) (Sf : set_func) (sigma : Substitution var (Term_ func var))
-      (x : var) (F : Form_ pred func var),
+    forall (Gamma : Con) (S : set_var) (Sf : sko_record) (sigma : Substitution var Term)
+      (x : var) (F : Form),
       (All F) \in Gamma -> isFresh x S -> hasTableau_ (Gamma ,, F{0 \to Free x}) S Sf sigma ->
       hasTableau_ Gamma (add x S) Sf sigma
 
    (** Delta rule *)
   | hasTableauNegAll :
-    forall (Gamma : Con_ pred func var) (S : set_var) (Sf : set_func) (sigma : Substitution var (Term_ func var))
-      (F : Form_ pred func var) (t : Term_ func var) (Hsko : is_sko t (Neg F) (fv Gamma) Sf),
+    forall (Gamma : Con) (S : set_var) (Sf : sko_record) (sigma : Substitution var Term)
+      (F : Form) (t : Term) (Hsko : is_sko t (Neg F) (fv Gamma) Sf),
       (Neg (All F)) \in Gamma -> hasTableau_ (Gamma ,, Neg F{0 \to t}) S Sf sigma ->
-      hasTableau_ Gamma S (add (symbol sko t Hsko) Sf) sigma.
+      hasTableau_ Gamma S (add_symbol (symbol sko t Hsko) F Sf) sigma.
 
-  Definition hasTableau (Gamma : Con_ pred func var) (sigma : Substitution var (Term_ func var)) : Prop :=
-    exists (S : set_var) (Sf : set_func), hasTableau_ Gamma S Sf sigma.
+  Definition hasTableau (Gamma : Con) (sigma : Substitution var Term) : Prop :=
+    exists (S : set_var) (Sf : sko_record), hasTableau_ Gamma S Sf sigma.
 End TableauxProofs.
 
 (* TODO: structural lemmas, e.g., strengthening, exchange law, (need something else?) *)
@@ -65,4 +71,11 @@ Section TableauxSoundness.
       hasTableau sko {{ Neg F }} sigma -> \models F.
   Proof.
     Admitted.
+
+(* Theorem hasTableau_sound : *)
+(*     forall (Gamma : Con_ pred func var) (sigma : Substitution var (Term_ func var)), *)
+(*       hasTableau sko Gamma sigma -> is_countersat (con_to_formula Gamma). *)
+(*   Proof. *)
+(*     intros ?? (S & Sf & htab). induction htab. *)
+(*     Admitted. *)
 End TableauxSoundness.
