theories/Skolemization.v
@@ -17,14 +17,27 @@ Section SkolemizationDef.
   Let set_var := set_atom var.
   Let set_func := set_atom func.
 
+  Class SkoRecord_ :=
+    { record :> Type
+    ; join : record -> record -> record
+    ; add_symbol : func -> Form_ pred func var -> record -> record
+    ; empty_record : record
+
+    ; join_unitr : forall (r : record), join r empty_record = r
+    ; join_unitl : forall (r : record), join empty_record r = r }.
+
   Class Skolemization_ :=
-    { is_sko :> Term_ func var -> Form_ pred func var -> set_var -> set_func -> Prop
+    { sko_record : SkoRecord_
+    ; is_sko :> Term_ func var -> Form_ pred func var -> set_var -> sko_record -> Prop
     ; symbol :
-        forall (t : Term_ func var) (F : Form_ pred func var) (S : set_var) (Sf : set_func),
+        forall (t : Term_ func var) (F : Form_ pred func var) (S : set_var) (Sf : sko_record),
           is_sko t F S Sf -> func }.
 End SkolemizationDef.
 
+Arguments SkoRecord_ : clear implicits.
+
 Arguments Skolemization_ : clear implicits.
+Arguments sko_record {_ _ _} _.
 Arguments is_sko {_ _ _ _} _ _ _ _.
 Arguments symbol {_ _ _} _ _ {_ _ _} _.
 
@@ -35,12 +48,26 @@ Section SkolemizationInstances.
   Let set_var := set_atom var.
   Let set_func := set_atom func.
 
+  (** An instance of [SkoRecord] with sets. *)
+  Definition sko_record_sets : SkoRecord_ pred func var.
+  Proof.
+    unshelve econstructor.
+    - exact set_func.
+    - exact union.
+    - exact empty_set.
+    - intros f _ r. exact (add f r).
+    - apply empty_unitr.
+    - apply empty_unitl.
+  Defined.
+
+  (* Use this function to avoid repeating the match on useless terms *)
   Definition gen_is_sko (t : Term_ func var) (P : func -> list (Term_ func var) -> Prop) : Prop :=
     match t with
     | Bound _ | Free _ => False
     | Fun f l => P f l
     end.
 
+  (* Use this function to get the skolem symbol (it abstracts away the impossible cases) *)
   Definition gen_symbol (t : Term_ func var) {P : func -> list (Term_ func var) -> Prop}
     (hsko : gen_is_sko t P) : func.
     refine
@@ -51,25 +78,37 @@ Section SkolemizationInstances.
     all: now rewrite e in hsko.
   Defined.
 
-  Instance OuterSkolemization : Skolemization_ pred func var :=
-    {| is_sko :=
-        fun t _ S Sf =>
-          gen_is_sko t (fun f l => (forall (x : var), mem (Free x) (from_list l) <-> mem x S) /\
-                                  isFresh f Sf)
+  Instance OuterSkolemization : Skolemization_ pred func var.
+  Proof.
+    unshelve econstructor.
+    - exact sko_record_sets. (* in outer skolemization, we only worry about freshness of the
+                                symbols *)
+    - intros t _ S Sf.
+      (* We want to check (i) that all the list [l] is composed of all the free variables of
+         the set [S], and (ii) that the symbol [f] is fresh in the set of skolem symbols already
+         appearing in the branch *)
+      exact (gen_is_sko t (fun f l => (forall (x : var), mem (Free x) (from_list l) <-> mem x S) /\
+                                     isFresh f Sf)).
+    - intros t ??? hsko. apply (gen_symbol t hsko).
+  Defined.
 
-    ;  symbol := fun t _ _ _ hsko => gen_symbol t hsko |}.
-
-  Instance InnerSkolemization : Skolemization_ pred func var :=
-    {| is_sko :=
-        fun t F _ Sf =>
-          gen_is_sko t (fun f l => (forall (x : var), mem (Free x) (from_list l) <-> mem x (fv F)) /\
-                                  isFresh f Sf)
-
-    ;  symbol := fun t _ _ _ hsko => gen_symbol t hsko |}.
+  Instance InnerSkolemization : Skolemization_ pred func var.
+  Proof.
+    unshelve econstructor.
+    - exact sko_record_sets. (* in inner skolemization, we also only care about freshness of the
+                                symbols *)
+    - intros t F _ Sf.
+      (* We want to check (i) that the list [l] is composed of all the free variables appearing
+         in the Skolemized formula [F], and (ii) that the symbol [f] is fresh in the set of
+         Skolem symbols already appearing in the branch. *)
+      exact (gen_is_sko t (fun f l => (forall (x : var), mem (Free x) (from_list l) <-> mem x (fv F)) /\
+                                     isFresh f Sf)).
+    - intros t ??? hsko. apply (gen_symbol t hsko).
+  Defined.
 End SkolemizationInstances.
 
 Module ConcreteSkolemizationInstances.
-  Import ConcreteSyntaxInstances.
+  Export ConcreteSyntaxInstances.
 
   Definition Skolemization := Skolemization_ string string string.
 
