examples/branching.v
@@ -1,0 +1,114 @@
+From Tableaux Require Import All.
+
+Import ATPCompat.
+
+(** In this file, we give an example of a tableau proof of the following branching
+    formula:
+      [exists x, P x -> P a /\ P b],
+    both in outer and inner Skolemization.
+
+    We start by defining the drinker formula using the extended syntax: *)
+Definition branching : EForm :=
+  EEx "x" (EImp (EPred "P" [EVar "x"])
+             (EAnd (EPred "P" [ EFun "a" [] ]) (EPred "P" [ EFun "b" [] ]))).
+
+(** In the proofs (be it in outer or in inner), we create two metavariables by instantiating
+    the formula twice, and replace one of them by [a] and the other one by [b].
+
+    Here, we do not create any new skolem symbol. *)
+Definition subst := translate_substitution [("X", EFun "a" []) ; ("X2", EFun "b" [])].
+
+Theorem outer_branching_proof :
+  hasTableau OuterSkolemization {{ translate_EForm (ENeg branching) }} subst.
+Proof.
+  (** As in the [drinker] formula, we need to give both (i) the set of free variables
+      of the tableau, and (ii) the set of Skolem symbols, which will be empty here. *)
+  exists \{ "X", "X2" \}, \{\}.
+
+  (** We start by creating a new free variable *)
+  eapply hasTableauNegEx with (i := 0).
+  1: reflexivity.
+  1: set_decide.
+
+  (** Then, the proof progresses as expected. *)
+  eapply hasTableauNegImp with (i := 0).
+  1: reflexivity.
+
+  (** Now, we have a branching rule. Here, we have to specify more things than simply the
+      index of the formula we want to use:
+
+      - we have to give the set of metavariables of each branch.
+        [S1] is the set of the left child, while [S2] is the set of the second child.
+        Note that, if one of them is empty, you cannot use [\{\}] as the elaboration process
+        does not understand that this is the notation for a set of strings. Instead, you should
+        use [@empty_set string _].
+      - we also have to give the set of skolem symbols of each branch. In outer skolemization,
+        this is a set, so we could use the same [@empty_set string _], but in general, it might
+        not be simply a set (e.g., in pre-inner Skolemization, where the formulas a symbol
+        originate from is important). Instead, for empty set of skolemization symbols, we
+        can use [empty_record]. *)
+  eapply hasTableauNegAnd with (S1 := @empty_set string _) (S2 := \{ "X2" \})
+                               (Sf1 := empty_record) (Sf2 := empty_record) (i := 1).
+  (** The first goal is, as always, [reflexivity]. *)
+  1: reflexivity.
+
+  (** The last three goals should always be automatically solved by [set_decide]. *)
+  3-5: set_decide.
+
+  (** Then, we can go into the different branches. First, let's do the left one. *)
+  { (** This is the branch where we have [Neg P a], hence we can directly conclude with the
+        contradiction using [P x]. *)
+    eapply hasTableauContr with (i := 2) (j := 0).
+    1: reflexivity.
+    1: reflexivity.
+    now esimpl. }
+
+  (** Next, let's do the right branch. *)
+  { (** Here, we have to create another metavariable [X2] to conclude using [Neg P b].
+        This is what we do with the first two rules. *)
+    eapply hasTableauNegEx with (i := 7).
+    1: reflexivity.
+    1: set_decide.
+
+    eapply hasTableauNegImp with (i := 0).
+    1: reflexivity.
+
+    (** Then, we can indeed use the contradiction between [P X2] and [Neg P b]. *)
+    eapply hasTableauContr with (i := 0) (j := 5).
+    1: reflexivity.
+    1: reflexivity.
+    now esimpl. }
+Qed.
+
+(** The proof in inner Skolemization is the same, as we have no Skolem symbol here. *)
+Theorem inner_branching_proof :
+  hasTableau InnerSkolemization {{ translate_EForm (ENeg branching) }} subst.
+Proof.
+  exists \{ "X", "X2" \}, \{\}.
+  eapply hasTableauNegEx with (i := 0).
+  1: reflexivity.
+  1: set_decide.
+
+  eapply hasTableauNegImp with (i := 0).
+  1: reflexivity.
+
+  eapply hasTableauNegAnd with (S1 := @empty_set string _) (S2 := \{ "X2" \})
+                               (Sf1 := empty_record) (Sf2 := empty_record) (i := 1).
+  1: reflexivity.
+  3-5: set_decide.
+  { eapply hasTableauContr with (i := 2) (j := 0).
+    1: reflexivity.
+    1: reflexivity.
+    now esimpl. }
+  { eapply hasTableauNegEx with (i := 7).
+    1: reflexivity.
+    1: set_decide.
+
+    eapply hasTableauNegImp with (i := 0).
+    1: reflexivity.
+
+    eapply hasTableauContr with (i := 0) (j := 5).
+    1: reflexivity.
+    1: reflexivity.
+    now esimpl. }
+Qed.
